updated some interfaces

fairness/examples/ticketlock/fair_lock.v
@@ -6,16 +6,73 @@ From trillium.fairness Require Import lemmas trace_len trace_lookup utils.
 From trillium.fairness.ext_models Require Import ext_models.
 
 
-Section FairLock.
-  Context {M: FairModel}.
-  
-  Context {allows_unlock: fmstate M -> fmstate M -> Prop}
-          {allows_lock: fmrole M -> fmstate M -> fmstate M -> Prop}.
-  
-  (* Context {AU_DEC: forall st, Decision (∃ st', allows_unlock st st')} *)
-  (*         {AL_DEC: forall st ρ, Decision (∃ st', allows_lock ρ st st')}.  *)
+Class FairLockPredicates (M: FairModel) := {
+  can_lock_st: fmrole M -> fmstate M -> Prop;
+  has_lock_st: fmrole M -> fmstate M -> Prop;
+  active_st: fmrole M -> fmstate M -> Prop;
+  state_wf: fmstate M -> Prop;
 
+  has_lock_st_dec :> forall ρ st, Decision (has_lock_st ρ st);
+  can_lock_st_dec :> forall ρ st, Decision (can_lock_st ρ st);
+  active_st_dec :> forall ρ st, Decision (active_st ρ st);
+}.
+
+
+Section FairLock.
+  Context `{FL: FairLockPredicates M}. 
+  Context {EM: ExtModel M}. 
+  
+  Let St := fmstate M.
+  Let R := fmrole M.
+  Let EFM := @ext_model_FM _ EM.
+
+  Definition eventual_release (tr: mtrace EFM) (ρ: R) (i: nat) :=
+    forall (ρ': R) j st' (JTH: tr S!! j = Some st')
+      (HAS_LOCK: has_lock_st ρ' st')
+      (AFTER: i <= j -> (ρ' ≠ ρ /\ forall k st_k (BETWEEN: i <= k <= j) (KTH: tr S!! k = Some st_k), ¬ has_lock_st ρ st_k)),
+      exists k st'', tr S!! k = Some st'' /\ j <= k /\ active_st ρ' st''.
+
+  Lemma eventual_release_strenghten tr ρ i (EV_REL: eventual_release tr ρ i):
+    forall (ρ': R) j st' (JTH: tr S!! j = Some st')
+      (HAS_LOCK: has_lock_st ρ' st')
+      (AFTER: i <= j -> (ρ' ≠ ρ /\ forall k st_k (BETWEEN: i <= k <= j) (KTH: tr S!! k = Some st_k), ¬ has_lock_st ρ st_k)),
+    exists k, ClassicalFacts.Minimal
+           (fun k => exists st'', tr S!! k = Some st'' /\ j <= k /\ active_st ρ' st'') k.
+  Proof using.
+    intros. red in EV_REL. specialize (EV_REL _ _ _ JTH HAS_LOCK AFTER).
+    destruct EV_REL as [k EV_REL]. pattern k in EV_REL.
+    eapply min_prop_dec in EV_REL; eauto.
+    intros.
+    destruct (tr S!! n) as [st | ] eqn:NTH.
+    2: { right. intros (? & ? & ?). congruence. }
+    destruct (decide (j <= n)).
+    2: { right. intros (? & ? & ?). lia. }
+    destruct (decide (active_st ρ' st)). 
+    - left. eauto.
+    - right. intros (? & ? & ? & ?). congruence.
+  Qed.
+      
+
+  Definition fair_lock_progress :=
+    forall (tr: mtrace EFM) (ρ: R) (i: nat) (st: St)
+      (VALID: mtrace_valid tr)
+      (FROM_INIT: forall st0, tr S!! 0 = Some st0 -> @state_wf _ FL st0)
+      (FAIR: inner_fair_ext_model_trace tr)
+      (ITH: tr S!! i = Some st)
+      (CAN_LOCK: can_lock_st ρ st)
+      (ACT: active_st ρ st)
+      (EV_REL: eventual_release tr ρ i),
+    exists n st', i < n /\ tr S!! n = Some st' /\ has_lock_st ρ st' /\ ¬ active_st ρ st'.
+  
+End FairLock.
+
+
+
+Section FairLockEM.
+  Context {M: FairModel}.
   Inductive fl_EI := flU | flL (ρ: fmrole M).
+  Context {au: fmstate M -> fmstate M -> Prop}
+          {al: fmrole M -> fmstate M -> fmstate M -> Prop}. 
 
   Global Instance fl_EI_dec: EqDecision fl_EI. 
   Proof using. solve_decision. Qed. 
@@ -34,87 +91,44 @@ Section FairLock.
     intros. destruct x; auto. by rewrite decode_encode_nat. 
   Qed.
 
-  Context (fl_active_exts: fmstate M -> gset fl_EI). 
-
   Definition fl_ETs (ι: fl_EI) :=
     match ι with
-    | flU => allows_unlock
-    | flL ρ => allows_lock ρ
+    | flU => au
+    | flL ρ => al ρ
     end.
 
-  Context (fl_active_exts_spec: 
-            forall st ι, ι ∈ fl_active_exts st <-> ∃ st', fl_ETs ι st st'). 
+  Context (fl_active_exts: fmstate M -> gset fl_EI).
+  Context (fl_active_exts_spec: forall st ι, ι ∈ fl_active_exts st <-> ∃ st', fl_ETs ι st st'). 
 
-  (* Context {EM: ExtModel M}. *)
-  Definition FL_EM: ExtModel M.
+
+  Definition FL_EM': ExtModel M.
     refine {| active_exts_spec := fl_active_exts_spec |}.
   Defined. 
 
-  Let St := fmstate M.
-  Let R := fmrole M.
-  Let EFM := @ext_model_FM _ FL_EM. 
+End FairLockEM.
 
-  Context (can_lock_st can_unlock_st has_lock_st active_st: R -> St -> Prop).
-  Context {active_st_Dec: forall ρ st, Decision (active_st ρ st)}. 
-  (* Context (is_init_st: St -> Prop). *)
-  Context (state_wf: St -> Prop). 
-  
-  Definition eventual_release (tr: mtrace EFM) (ρ: R) (i: nat) :=
-    forall (ρ': R) j st' (JTH: tr S!! j = Some st')
-      (HAS_LOCK: has_lock_st ρ' st')
-      (AFTER: i <= j -> (ρ' ≠ ρ /\ forall k st_k (BETWEEN: i <= k <= j) (KTH: tr S!! k = Some st_k), ¬ has_lock_st ρ st_k)),
-      exists k st'', tr S!! k = Some st'' /\ j <= k /\ active_st ρ' st''.
 
-  Lemma eventual_release_strenghten tr ρ i (EV_REL: eventual_release tr ρ i):
-    forall (ρ': R) j st' (JTH: tr S!! j = Some st')
-      (HAS_LOCK: has_lock_st ρ' st')
-      (AFTER: i <= j -> (ρ' ≠ ρ /\ forall k st_k (BETWEEN: i <= k <= j) (KTH: tr S!! k = Some st_k), ¬ has_lock_st ρ st_k)),
-    exists k, ClassicalFacts.Minimal
-           (fun k => exists st'', tr S!! k = Some st'' /\ j <= k /\ active_st ρ' st'') k.
-  Proof using active_st_Dec.
-    intros. red in EV_REL. specialize (EV_REL _ _ _ JTH HAS_LOCK AFTER).
-    destruct EV_REL as [k EV_REL]. pattern k in EV_REL.
-    eapply min_prop_dec in EV_REL; eauto.
-    intros.
-    destruct (tr S!! n) as [st | ] eqn:NTH.
-    2: { right. intros (? & ? & ?). congruence. }
-    destruct (decide (j <= n)).
-    2: { right. intros (? & ? & ?). lia. }
-    destruct (active_st_Dec ρ' st).
-    - left. eauto.
-    - right. intros (? & ? & ? & ?). congruence.
-  Qed.
-      
+Class FairLockExt (M: FairModel) := {
+  allows_unlock: fmstate M -> fmstate M -> Prop;
+  allows_lock: fmrole M -> fmstate M -> fmstate M -> Prop;
+  fl_active_exts: fmstate M -> gset (@fl_EI M);
+  fl_active_exts_spec: forall st ι, ι ∈ fl_active_exts st <-> ∃ st', (@fl_ETs _ allows_unlock allows_lock) ι st st';
+}.
 
-  Definition fair_lock_progress :=
-    forall (tr: mtrace EFM) (ρ: R) (i: nat) (st: St)
-      (VALID: mtrace_valid tr)
-      (FROM_INIT: forall st0, tr S!! 0 = Some st0 -> state_wf st0)
-      (FAIR: inner_fair_ext_model_trace tr)
-      (ITH: tr S!! i = Some st)
-      (CAN_LOCK: can_lock_st ρ st)
-      (ACT: active_st ρ st)
-      (EV_REL: eventual_release tr ρ i),
-    exists n st', i < n /\ tr S!! n = Some st' /\ has_lock_st ρ st' /\ ¬ active_st ρ st'.
-  
 
-  (* TODO: mention these function equivalents of relations
-           in the definition of EM itself? *)
-  Class FairLock := {
-      lock_progress: fair_lock_progress;
+Definition FL_EM `(FLE: FairLockExt M) :=
+  @FL_EM' M allows_unlock allows_lock fl_active_exts fl_active_exts_spec. 
 
-      allow_unlock_impl: fmstate M -> fmstate M;
-      allow_lock_impl: fmrole M -> fmstate M -> fmstate M;
-      allows_unlock_impl_spec st (WF: state_wf st):
-      forall st', allows_unlock st st' <-> 
-              (allow_unlock_impl st = st' /\ (exists ρ, has_lock_st ρ st /\ ¬ active_st ρ st));
-      allows_lock_impl_spec ρ st:
-      forall st', allows_lock ρ st st' <-> 
-              (allow_lock_impl ρ st = st' /\ (can_lock_st ρ st /\ ¬ active_st ρ st));
 
-      has_lock_st_dec :> forall ρ st, Decision (has_lock_st ρ st);
-      can_lock_st_dec :> forall ρ st, Decision (can_lock_st ρ st);
-      active_st_dec :> forall ρ st, Decision (active_st ρ st);
-  }.
+Class FairLock (M: FairModel) (FLP: FairLockPredicates M) (FLE: FairLockExt M) := {
+  allow_unlock_impl: fmstate M -> fmstate M;
+  allow_lock_impl: fmrole M -> fmstate M -> fmstate M;
+  allows_unlock_impl_spec st (WF: state_wf st):
+    forall st', allows_unlock st st' <->
+             (allow_unlock_impl st = st' /\ (exists ρ, has_lock_st ρ st /\ ¬ active_st ρ st));
+  allows_lock_impl_spec ρ st:
+    forall st', allows_lock ρ st st' <->
+             (allow_lock_impl ρ st = st' /\ (can_lock_st ρ st /\ ¬ active_st ρ st));
 
-End FairLock.
+  lock_progress: @fair_lock_progress _ FLP (FL_EM FLE);
+}.
